unnecessary axioms removed, messages->steps

flp.v
@@ -4,7 +4,6 @@
 (** also constructive proofs: http://citeseerx.ist.psu.edu/viewdoc/download?doi=10.1.1.221.7907&rep=rep1&type=pdf **)
 (** and http://www.cs.cornell.edu/courses/cs7412/2011sp/ConsensusRebecca.pdf **)
 
-
 Require Import Arith.
 Require Import List.
 Require Import Coq.Logic.Classical.
@@ -26,8 +25,6 @@ end.
 
 Definition Configuration := list Process.
 
-Axiom CfgSize: forall cfg:Configuration, length cfg >= 2.
-
 Definition decidedValue(cfg:Configuration)(b:Binary):Prop := In (FinishedProcess b) cfg.
 
 Definition decided(cfg:Configuration):Prop := decidedValue cfg true \/ decidedValue cfg false.
@@ -44,16 +41,9 @@ Definition Schedule := list nat.
 
 Parameter chooseFn : Configuration -> nat -> Process.
 
-(** Parameter sameProcess: Process -> Process -> Prop. **)
-
-Axiom chooseIn : forall cfg msg, In (chooseFn cfg msg) cfg.
-
-Axiom stepForEveryProcess1: forall cfg p, In p cfg -> exists msg, chooseFn cfg msg = p.
-Axiom stepForEveryProcess2: forall cfg p, In p cfg -> exists msg, chooseFn cfg msg <> p.
 
 (** Configuration transition function **)
 Parameter eventFn : Configuration -> nat -> Configuration.
-
 
 
 (** There's no change in deciding value **)
@@ -63,11 +53,11 @@ Axiom Termination: forall cfg b msg, decidedValue cfg b -> decidedValue (eventFn
 Fixpoint run (cfg:Configuration)(s:Schedule): Configuration :=
 match s with
 | nil => cfg
-| cons msg t => eventFn (run cfg t) msg
+| cons step t => eventFn (run cfg t) step
 end.  
 
 (** todo: proove? **)
-Axiom RunCommutativity: forall cfg msg s, run (run cfg [msg]) s = run cfg (msg :: s).
+Axiom RunCommutativity: forall cfg step s, run (run cfg [step]) s = run cfg (step :: s).
 
 
 Lemma Termination1: forall cfg b s, decidedValue cfg b -> decidedValue (run cfg s) b.
@@ -84,13 +74,6 @@ Qed.
 to the properties of consensus **)
 Definition deciding(cfg:Configuration)(s:Schedule): Prop := decided (run cfg s).
 
-Hypothesis InitialConfiguration: Configuration.
-
-
-Axiom InitialNoConsensus: ~decided InitialConfiguration.
-Axiom TrueReacheable: exists s1, decidedValue (run InitialConfiguration s1) true.
-Axiom FalseReacheable: exists s2, decidedValue (run InitialConfiguration s2) false.
-
 
 Definition univalent_true(cfg:Configuration):= 
   (exists s1, decidedValue(run cfg s1) true) /\ ~(exists s2, decidedValue (run cfg s2) false).
@@ -104,10 +87,8 @@ Definition bivalent(cfg:Configuration):= (~ decided cfg) /\
   (exists s1, decidedValue (run cfg s1) false) /\ (exists s2, decidedValue (run cfg s2) true).
 
 
-
 (** "By the total correctness of P, and the fact that there are always admissible runs, V > 0" **)
 Axiom Correctness: forall cfg, bivalent cfg \/ univalent cfg.
-
 
 
 Lemma UnNotBiv: forall cfg, univalent cfg <-> ~ bivalent cfg.
@@ -123,7 +104,6 @@ tauto.
 Qed.
 
 
-
 Lemma BivNotUn: forall cfg, bivalent cfg <-> ~ univalent cfg.
 Proof.
 intros.
@@ -135,7 +115,6 @@ pose proof Correctness as C.
 specialize (C cfg).
 tauto.
 Qed.
-
 
 
 Lemma BivalentPaths: forall cfg, bivalent cfg ->
@@ -172,11 +151,11 @@ specialize (C (run (run cfg x0) x1)).
 auto.
 Qed.
 
+
 (** todo: prove **)
 Axiom BivalentPaths2: forall cfg, bivalent cfg ->
   (exists st1 s1, univalent_false(run cfg (st1::s1))) /\ 
   (exists st2 s2, univalent_true(run cfg (st2::s2))).
-
 
 
 
@@ -198,6 +177,7 @@ unfold univalent_true in B.
 unfold bivalent in B.
 tauto.
 Qed.
+
 
 Lemma UnTNotBiv: forall cfg, univalent_true cfg -> ~ bivalent cfg.
 Proof.
@@ -262,49 +242,49 @@ Axiom Correctness8: forall cfg st s, univalent_false (run cfg (st :: s)) ->
 (** todo: prove ! **)
 Axiom Correctness9: forall cfg st s, univalent_true (run cfg (st :: s)) -> bivalent (run cfg [st]) \/ univalent_true (run cfg [st]).
 
-Axiom Async1: forall cfg msg1 msg2, (chooseFn cfg msg1) <>  (chooseFn cfg msg2) -> 
-  run cfg ([msg1;msg2]) = run cfg ([msg2;msg1]).
+Axiom Async1: forall cfg step1 step2, (chooseFn cfg step1) <>  (chooseFn cfg step2) -> 
+  run cfg ([step1;step2]) = run cfg ([step2;step1]).
 
 
 
 Axiom Decidability: forall cfg n1 n2, chooseFn cfg n1 = chooseFn cfg n2 \/ chooseFn cfg n1 <> chooseFn cfg n2.
 
 
-Lemma OneStepLemmaP1: forall cfg msg1 msg2, 
-  chooseFn cfg msg1 <> chooseFn cfg msg2 /\ 
-    univalent_false (run cfg [msg1]) /\
-    univalent_true (run cfg [msg2])-> False.
+Lemma OneStepLemmaP1: forall cfg step1 step2, 
+  chooseFn cfg step1 <> chooseFn cfg step2 /\ 
+    univalent_false (run cfg [step1]) /\
+    univalent_true (run cfg [step2])-> False.
 Proof.
 intuition.
 pose proof RunCommutativity as RC.
 specialize(RC cfg).
 pose proof Async1 as A1.
-specialize(A1 cfg msg1 msg2).
+specialize(A1 cfg step1 step2).
 pose proof Correctness6 as C6.
 pose proof Correctness7 as C7.
-specialize (C6 (run cfg [msg2]) [msg1]).
+specialize (C6 (run cfg [step2]) [step1]).
 rewrite RC in C6.
-specialize (C7 (run cfg [msg1]) [msg2]).
+specialize (C7 (run cfg [step1]) [step2]).
 rewrite RC in C7.
 intuition.
 rewrite H1 in H3.
 pose proof Correctness3 as C3.
-specialize(C3 (run cfg [msg2; msg1])).
+specialize(C3 (run cfg [step2; step1])).
 tauto.
 Qed.
 
-Lemma OneStepLemmaP2: forall cfg msg1 msg2,  
-    univalent_false (run cfg [msg1]) /\
-    univalent_true (run cfg [msg2]) -> chooseFn cfg msg1 = chooseFn cfg msg2.
+Lemma OneStepLemmaP2: forall cfg step1 step2,  
+    univalent_false (run cfg [step1]) /\
+    univalent_true (run cfg [step2]) -> chooseFn cfg step1 = chooseFn cfg step2.
 Proof.
-intros cfg msg1 msg2.
+intros cfg step1 step2.
 pose proof OneStepLemmaP1 as P1.
-specialize(P1 cfg msg1 msg2).
+specialize(P1 cfg step1 step2).
 tauto.
 Qed.
 
-(** todo: rename Message -> Step, msg -> step **)
-Axiom AnotherProcessStepExists: forall cfg msg, exists msg0, chooseFn cfg msg <> chooseFn cfg msg0. 
+(** todo: rename Message -> Step, step-> step **)
+Axiom AnotherProcessStepExists: forall cfg step, exists step0, chooseFn cfg step <> chooseFn cfg step0. 
 Parameter randomStep: Configuration -> nat.
 
 
@@ -326,21 +306,21 @@ unfold univalent.
 tauto.
 Qed.
 
-Lemma OtherBivalent: forall cfg msg1 msg2, (chooseFn cfg msg1 = chooseFn cfg msg2 /\ 
-  univalent_true (run cfg [msg1]) /\ univalent_false (run cfg [msg2])) -> 
-  forall msg, chooseFn cfg msg <> chooseFn cfg msg1 -> bivalent (run cfg [msg]).
+Lemma OtherBivalent: forall cfg step1 step2, (chooseFn cfg step1 = chooseFn cfg step2 /\ 
+  univalent_true (run cfg [step1]) /\ univalent_false (run cfg [step2])) -> 
+  forall step, chooseFn cfg step <> chooseFn cfg step1 -> bivalent (run cfg [step]).
 Proof.
 intuition.
 apply BivNotUn.
 unfold univalent.
 pose proof OneStepLemmaP1 as P1.
 intuition.
-(** CASE : univalent_true (run cfg [msg]) **)
-assert(P1T := P1 cfg msg2 msg).
+(** CASE : univalent_true (run cfg [step]) **)
+assert(P1T := P1 cfg step2 step).
 rewrite H0 in H1.
 auto.
-(** CASE : univalent_false (run cfg [msg]) **)
-assert(P1H := P1 cfg msg msg1).
+(** CASE : univalent_false (run cfg [step]) **)
+assert(P1H := P1 cfg step step1).
 auto.
 Qed. 
 
@@ -348,17 +328,17 @@ Qed.
 (** only the same process could goes to univalent_true & univalent_false states, so we choose another process and
 it must be bivalent as proven by the OtherBivalent lemma **)
 
-Lemma OneStepLemmaP3: forall cfg msg1 msg2, univalent_true (run cfg [msg1]) /\ univalent_false (run cfg [msg2]) -> 
-  exists msg : nat, bivalent (run cfg [msg]).  
+Lemma OneStepLemmaP3: forall cfg step1 step2, univalent_true (run cfg [step1]) /\ univalent_false (run cfg [step2]) -> 
+  exists step: nat, bivalent (run cfg [step]).  
 Proof.
 intros.
 pose proof OneStepLemmaP2 as P2.
-specialize(P2 cfg msg2 msg1).
+specialize(P2 cfg step2 step1).
 intuition.
-assert(AP := AnotherProcessStepExists cfg msg1).
+assert(AP := AnotherProcessStepExists cfg step1).
 destruct AP.
 pose proof OtherBivalent as OB.
-specialize (OB cfg msg1 msg2).
+specialize (OB cfg step1 step2).
 intuition.
 rewrite H in H3.
 intuition.
@@ -368,8 +348,9 @@ exists x.
 assumption.
 Qed.
 
+(** The main lemma, named OneStepLemma after Constable's paper **)
 
-Theorem OneStepLemma: forall cfg, bivalent cfg -> exists msg, bivalent (run cfg [msg]).
+Theorem OneStepLemma: forall cfg, bivalent cfg -> exists step, bivalent (run cfg [step]).
 Proof.
 intros.
 assert(S := randomStep cfg).
@@ -414,6 +395,8 @@ specialize(P3 cfg x S).
 tauto.
 Qed.
 
+(** Not strictly corresponding to the original paper, as there's no any 
+process & event considered **)
 
 Theorem FLP_Lemma3: forall cfg, bivalent cfg -> forall m, exists s, length s > m -> bivalent (run cfg s).
 Proof.
@@ -428,7 +411,16 @@ apply H0.
 Qed.
 
 
+(** Initial Configuration & its properties **)
+
+Parameter InitialConfiguration: Configuration.
+
+Axiom InitialNoConsensus: ~decided InitialConfiguration.
+Axiom TrueReacheable: exists s1, decidedValue (run InitialConfiguration s1) true.
+Axiom FalseReacheable: exists s2, decidedValue (run InitialConfiguration s2) false.
+
 (** Lemma 2 from original paper **)
+(** Initial configuration is bivalent **)
 Theorem FLP_Lemma2: bivalent(InitialConfiguration).
 Proof.
 pose proof InitialNoConsensus as I.
